src/proof/text/String.v
@@ -93,7 +93,7 @@ Proof.
   { iExists ls. iSplitR; first by iPureIntro. iFrame "Htextr". by iPureIntro. }
   wp_auto.
   wp_apply (wp_Store__runlock with "[$His_store $Hrlo Hseq Hpool]").
-  { iFrame "Hseq". rewrite /own_type_pool_runs. iSplitR; [by iPureIntro | iFrame "Hpool"]. }
+  { iFrame "Hseq". rewrite /own_type_pool. iSplitR; [by iPureIntro | iFrame "Hpool"]. }
   iIntros "Hcap".
   wp_auto.
   have Hfst : (runs_model (tm_runs tm)).*1 = tm_arr tm.
